lib/coq/caduceus_lists.v
@@ -33,34 +33,34 @@ Implicit Arguments In_app_cons [A].
 
 (** the Coq pointer list associated to a (finite) linked list *)
 
-Definition plist (Z:Set) := list (pointer Z).
+Definition plist (R:Set) := list (pointer R).
 
-Definition in_list (Z:Set) := (@In (pointer Z)).
+Definition in_list (R:Set) := (@In (pointer R)).
 
 (** * Paths *)
 
 Section Paths.
 
-Variable Z: Set.
+Variable R: Set.
 
 (** [(lpath t p1 l p2)] :
     there is a path from pointer [p1] to pointer [p2] using links in store [t],
     and the list of pointers along this path is [l]. *)
 
-Inductive lpath (a: alloc_table)  (next: pointer Z -> pointer Z) : 
-      pointer Z -> plist Z -> pointer Z -> Prop :=
-  | Path_null : forall p:pointer Z, lpath a next p nil p
+Inductive lpath (a: alloc_table)  (next: pointer R -> pointer R) : 
+      pointer R -> plist R -> pointer R -> Prop :=
+  | Path_null : forall p:pointer R, lpath a next p nil p
   | Path_cons :
-      forall p1 p2:pointer Z,
+      forall p1 p2:pointer R,
         ~(p1 = null) -> valid a p1 ->
-        forall l:list (pointer Z),
+        forall l:list (pointer R),
           lpath a next (next p1) l p2 -> lpath a next  p1 (cons p1 l) p2.
 
 Hint Constructors lpath.
 
 Lemma lpath_eq_fun : 
-  forall (a: alloc_table) (f g :pointer Z -> pointer Z) (p q: pointer Z)
-(l : list (pointer Z)),
+  forall (a: alloc_table) (f g :pointer R -> pointer R) (p q: pointer R)
+(l : list (pointer R)),
  (forall p, In p l -> f p = g p) ->
  lpath a f p l q  -> lpath a g p l q
 .
@@ -81,8 +81,8 @@ Qed.
 (** [(llist t p l)]: there is a (finite) linked list starting from pointer [p]
     using links in store [t], and this list of pointers is [l] *)
 
-Definition llist (a: alloc_table) (next : pointer Z -> pointer Z) (p:pointer Z) 
-  (l:plist Z) :=
+Definition llist (a: alloc_table) (next : pointer R -> pointer R) (p:pointer R) 
+  (l:plist R) :=
   lpath a next p l null.
 
 Hint Unfold llist .
@@ -91,21 +91,21 @@ Hint Unfold llist .
     inductive definition of [llist])  *)
 
 Lemma llist_null :
- forall (a: alloc_table) (next : pointer Z -> pointer Z) (p:pointer Z), 
+ forall (a: alloc_table) (next : pointer R -> pointer R) (p:pointer R), 
   llist a next p nil -> p = null.
 Proof.
 unfold llist; inversion 1; trivial.
 Qed.
 
 Lemma llist_cons :
- forall (a: alloc_table) (next : pointer Z -> pointer Z) (p1 p2:pointer Z) (l:plist Z),
+ forall (a: alloc_table) (next : pointer R -> pointer R) (p1 p2:pointer R) (l:plist R),
    llist a next p1 (cons p2 l) -> p1 = p2 /\ llist a next (next p2) l.
 Proof.
 unfold llist; inversion 1; intuition.
 Qed.
 
 Lemma llist_head :
- forall (a: alloc_table) (next : pointer Z -> pointer Z) (p1 p2:pointer Z) (l:plist Z),
+ forall (a: alloc_table) (next : pointer R -> pointer R) (p1 p2:pointer R) (l:plist R),
    llist a next p1 (cons p2 l) -> p1 = p2.
 Proof.
 unfold llist; inversion 1; intuition.
@@ -114,14 +114,14 @@ Qed.
 Hint Resolve llist_head.
 
 Lemma llist_start :
- forall (a: alloc_table) (next : pointer Z -> pointer Z ) (p1:pointer Z) (l:plist Z),
+ forall (a: alloc_table) (next : pointer R -> pointer R ) (p1:pointer R) (l:plist R),
    llist a next p1 l -> p1 <> null -> l = p1 :: tail l.
 Proof.
 unfold llist; inversion 1; intuition.
 Qed.
 
 Lemma llist_head_non_null :
- forall (a: alloc_table) (next : pointer Z-> pointer Z) (p1 p2:pointer Z) (l:plist Z),
+ forall (a: alloc_table) (next : pointer R-> pointer R) (p1 p2:pointer R) (l:plist R),
    llist a next p1 (cons p2 l) -> p1 <> null.
 Proof.
 unfold llist; inversion 1; intuition.
@@ -130,9 +130,9 @@ Qed.
 (** invariance of a list when updating a cell outside of this list *)
 
 Lemma lpath_pset_same :
- forall (a: alloc_table) (m : memory (pointer Z) Z) (p p':pointer Z) (l:plist Z),
+ forall (a: alloc_table) (m : memory (pointer R) R) (p p':pointer R) (l:plist R),
    lpath a (acc m) p l p' ->
-   forall p1 p2:pointer Z,
+   forall p1 p2:pointer R,
      ~ In p1 l -> lpath a (acc (upd m p1 p2)) p l p'.
 Proof.
 simple induction 1; intuition.
@@ -145,9 +145,9 @@ Qed.
 Hint Resolve lpath_pset_same .
 
 Lemma llist_pset_same :
- forall (a: alloc_table) (m : memory (pointer Z) Z) (p:pointer Z) (l:plist Z),
+ forall (a: alloc_table) (m : memory (pointer R) R) (p:pointer R) (l:plist R),
    llist a (acc m) p l ->
-   forall p1 p2:pointer Z,
+   forall p1 p2:pointer R,
      ~ In p1 l -> llist a (acc (upd m p1 p2)) p l.
 Proof.
 unfold llist; intros; apply lpath_pset_same; auto.
@@ -157,7 +157,7 @@ Hint Resolve llist_pset_same .
 (** [llist] is a function *)
 
 Lemma llist_function :
- forall (a a': alloc_table) (next : pointer Z -> pointer Z) (l1 l2:plist Z) (p:pointer Z),
+ forall (a a': alloc_table) (next : pointer R -> pointer R) (l1 l2:plist R) (p:pointer R),
    llist a next p l1 -> llist a' next p l2 -> l1 = l2.
 Proof.
 (* induction l1; intuition. *)
@@ -180,9 +180,9 @@ Qed.
 Implicit Arguments llist_function.
 
 Lemma llist_append :
- forall (a: alloc_table) (next : pointer Z -> pointer Z) (l1 l2:plist Z) (p:pointer Z),
+ forall (a: alloc_table) (next : pointer R -> pointer R) (l1 l2:plist R) (p:pointer R),
    llist a next p (app l1 l2) ->
-    exists p' : pointer Z, lpath a next p l1 p' /\ llist a next p' l2.
+    exists p' : pointer R, lpath a next p l1 p' /\ llist a next p' l2.
 Proof.
 simple induction l1; simpl; intuition.
 exists p; auto.
@@ -213,7 +213,7 @@ Qed.
 (** a list starting with [p] does not contain [p] in its remaining elements *)
 
 Lemma llist_not_starting :
- forall (a: alloc_table) (next: pointer Z -> pointer Z) (p:pointer Z) (l:plist Z),
+ forall (a: alloc_table) (next: pointer R -> pointer R) (p:pointer R) (l:plist R),
    llist a next (next p) l -> ~ In p l.
 Proof.
 red; intros.
@@ -228,8 +228,8 @@ rewrite length_app; simpl; omega.
 Qed.
 
 Lemma llist_no_rep: 
-  forall (a : alloc_table)(next : pointer Z ->pointer Z)(p q : pointer Z)
-(l : plist Z) , llist a next p (q :: l) -> p=q /\ ~ In p l.
+  forall (a : alloc_table)(next : pointer R ->pointer R)(p q : pointer R)
+(l : plist R) , llist a next p (q :: l) -> p=q /\ ~ In p l.
 unfold llist.
 intros.
 inversion H.
@@ -242,27 +242,27 @@ Qed.
 (** * Finite lists characterization *)
 
 (*
-Inductive is_list (a: alloc_table) (next: pointer Z -> pointer Z) : 
-   pointer Z -> Prop :=
+Inductive is_list (a: alloc_table) (next: pointer R -> pointer R) : 
+   pointer R -> Prop :=
   | List_null : is_list a next null
   | List_cons :
-      forall p:pointer Z,
+      forall p:pointer R,
         ~(p = null) -> valid a p -> is_list a next (next p) -> is_list a next p.
 
 Hint Constructors is_list.
 
 Lemma is_list_llist :
- forall (a: alloc_table) (next: pointer Z -> pointer Z) (p:pointer Z),
-   is_list a next p -> exists l : plist Z, llist a next p l.
+ forall (a: alloc_table) (next: pointer R -> pointer R) (p:pointer R),
+   is_list a next p -> exists l : plist R, llist a next p l.
 Proof.
 intros; elim H.
-exists (nil (A:=pointer Z)); intuition.
+exists (nil (A:=pointer R)); intuition.
 intros. elim H3; intros.
 exists (cons p0 x); intuition.
 Qed.
 
 Lemma llist_is_list :
- forall (a: alloc_table) (next: pointer Z -> pointer Z) (l:plist Z) (p:pointer Z),
+ forall (a: alloc_table) (next: pointer R -> pointer R) (l:plist R) (p:pointer R),
    llist a next p l -> is_list a next p.
 Proof.
 simple induction l; intuition.
@@ -271,21 +271,21 @@ inversion H0; intuition.
 Qed.
 *)
 
-Definition is_list a next p := exists l : plist Z, llist a next p l.
+Definition is_list a next p := exists l : plist R, llist a next p l.
 
 (** * WF relation over linked lists *)
 
 
-Definition Length := ((memory (pointer Z) Z) * (pointer Z))%type.
+Definition Length := ((memory (pointer R) R) * (pointer R))%type.
 Definition length (a: alloc_table)
-   (t : memory (pointer Z) Z) (p:pointer Z) := (t, p).
+   (t : memory (pointer R) R) (p:pointer R) := (t, p).
 
-Definition length_order (c1 c2: memory (pointer Z) Z * pointer Z) : Prop :=
+Definition length_order (c1 c2: memory (pointer R) R * pointer R) : Prop :=
   let (t1, p1) := c1 in
   let (t2, p2) := c2 in
     exists a : alloc_table,
-    exists l1 : plist Z,
-    exists l2 : plist Z,
+    exists l1 : plist R,
+    exists l2 : plist R,
     llist a (acc t1) p1 l1 /\ llist a (acc t2) p2 l2 /\ (List.length l1 < List.length l2)%nat.
 
 Lemma length_order_wf : well_founded length_order.
@@ -294,7 +294,7 @@ apply well_founded_inv_lt_rel_compat with
  (F := fun (x:Length) n =>
          let (t, p) := x in
          exists a : alloc_table,
-         exists l : plist Z, llist a (acc t) p l /\ List.length l = n).
+         exists l : plist R, llist a (acc t) p l /\ List.length l = n).
 unfold length_order, inv_lt_rel.
 simple destruct x; simple destruct y; intuition.
 elim H; clear H; intros a H; elim H; clear H;
@@ -424,11 +424,11 @@ Admitted.
 End Cyclicity.
 *)
 
-Axiom eq_pointer_dec : forall p1 p2 : pointer Z, {p1 = p2} + {p1 <> p2}.
+Axiom eq_pointer_dec : forall p1 p2 : pointer R, {p1 = p2} + {p1 <> p2}.
 
 Section NoRepetition.
 
-Fixpoint no_rep (l:plist Z) {struct l}: Prop :=
+Fixpoint no_rep (l:plist R) {struct l}: Prop :=
 match l with
 | nil => True
 | (a::l) => (if In_dec eq_pointer_dec a l then False else True)  /\ no_rep l
@@ -446,7 +446,7 @@ Qed.
 Implicit Arguments split_list.
 
 Lemma no_rep_sublist1 :
- forall (l : plist Z)(p:pointer Z),
+ forall (l : plist R)(p:pointer R),
   no_rep (p::l) -> no_rep l.
 intros.
 destruct H.
@@ -454,7 +454,7 @@ apply H0.
 Qed.
 
 Lemma no_rep_sublist :
-  forall (l l1 l2 : plist Z),
+  forall (l l1 l2 : plist R),
   no_rep l -> l = l1 ++ l2 -> no_rep l2.
 induction l.
 intros.
@@ -475,7 +475,7 @@ Qed.
 
 Ltac caseq t := generalize (refl_equal t);pattern t at -1;case t.
 
-Lemma no_rep_p : forall (p1:pointer Z)(lp: plist Z), no_rep(p1::lp)->
+Lemma no_rep_p : forall (p1:pointer R)(lp: plist R), no_rep(p1::lp)->
 ~In p1 lp.
 intros.
 simpl in H.
@@ -489,7 +489,7 @@ intros i.
 elim (i H0).
 Qed.
 
-Lemma no_rep_sublist2 : forall (l l1 l2 : plist Z) (a : pointer Z), no_rep l ->
+Lemma no_rep_sublist2 : forall (l l1 l2 : plist R) (a : pointer R), no_rep l ->
 l = l1 ++a::l2 -> no_rep (l1++l2).
 induction l.
 intros.
@@ -520,7 +520,7 @@ intuition.
 apply IHl with a0;auto.
 Qed.
 
-Lemma no_rep_sublist_bis : forall (l2 l l1  : plist Z), no_rep l ->
+Lemma no_rep_sublist_bis : forall (l2 l l1  : plist R), no_rep l ->
 l = l1 ++ l2 -> no_rep l1.
 induction l2.
 intros.
@@ -536,7 +536,7 @@ intro.
 apply IHl2 with (l1++l2);auto.
 Qed.
 
-Lemma no_rep_false : forall (p1 : pointer Z)(lp : plist Z),
+Lemma no_rep_false : forall (p1 : pointer R)(lp : plist R),
 no_rep (p1 :: p1 :: lp) -> False.
 intros.
 unfold no_rep in H; fold no_rep in H.
@@ -544,7 +544,7 @@ inversion_clear H as [H0 H1].
 destruct (In_dec eq_pointer_dec p1 (p1 :: lp)); auto with *.
 Qed.
 
-Lemma no_rep_false2 : forall (p1 : pointer Z)(lp1 lp2 : plist Z),
+Lemma no_rep_false2 : forall (p1 : pointer R)(lp1 lp2 : plist R),
 no_rep (p1 ::lp1 ++ p1 :: lp2) -> False.
 intros.
 simpl in H.
@@ -558,7 +558,7 @@ simpl;left;auto.
 right;auto.
 Qed.
 
-Lemma no_rep_p_bis : forall (p1:pointer Z)(lp1 lp2:plist Z), no_rep(lp1++p1::lp2)->
+Lemma no_rep_p_bis : forall (p1:pointer R)(lp1 lp2:plist R), no_rep(lp1++p1::lp2)->
 ~In p1 lp1.
 intros.
 intro.
@@ -577,12 +577,12 @@ Qed.
 
 
 Lemma no_rep_in_app :
-  forall p : pointer Z,
-  forall lp1 lp2a lp2b : plist Z,
+  forall p : pointer R,
+  forall lp1 lp2a lp2b : plist R,
   no_rep (p::lp1) -> no_rep (lp2a++p::lp2b) ->
-  (forall q : pointer Z,
+  (forall q : pointer R,
      In q (p::lp1) -> In q (lp2a++p::lp2b)) ->
-  forall q : pointer Z, In q lp1 -> In q (lp2a ++ lp2b).
+  forall q : pointer R, In q lp1 -> In q (lp2a ++ lp2b).
 intros.
 case (eq_pointer_dec q p).
 intro.
@@ -604,7 +604,7 @@ apply H1.
 right;auto.
 Qed.
 
-Lemma no_rep_sublist3 : forall (l l1 l2 : plist Z) ( a : pointer Z), no_rep l ->
+Lemma no_rep_sublist3 : forall (l l1 l2 : plist R) ( a : pointer R), no_rep l ->
 l = l1 ++a::l2 -> no_rep (a::l1++l2).
 induction l as [ | p1 l].
 intros l1 l2 a _ H; destruct l1; simpl in H; discriminate.
@@ -627,12 +627,12 @@ apply no_rep_sublist2 with (p1' :: l1 ++ a :: l2) a; trivial.
 Qed.
 
 Lemma no_rep_in_app2 :
-  forall p : pointer Z,
-  forall lp1 lp2a lp2b : plist Z,
+  forall p : pointer R,
+  forall lp1 lp2a lp2b : plist R,
   no_rep (p::lp1) -> no_rep (lp2a++p::lp2b) ->
-  (forall q : pointer Z,
+  (forall q : pointer R,
     In q (lp2a++p::lp2b) -> In q (p::lp1)) ->
-  forall q : pointer Z, In q (lp2a ++ lp2b) -> In q lp1.
+  forall q : pointer R, In q (lp2a ++ lp2b) -> In q lp1.
 intros.
 case (eq_pointer_dec q p).
 intro.
@@ -668,7 +668,7 @@ End NoRepetition.
 
 (* consecutives pairs in a list *)
 
-Fixpoint pair_in_list (p1:pointer Z) (p2:pointer Z)(l: plist Z) {struct l} : Prop :=
+Fixpoint pair_in_list (p1:pointer R) (p2:pointer R)(l: plist R) {struct l} : Prop :=
   match l with
   | nil => False
   | b :: m => (b = p1 /\ match  m with
@@ -679,7 +679,7 @@ Fixpoint pair_in_list (p1:pointer Z) (p2:pointer Z)(l: plist Z) {struct l} : Pro
   end.
 
 Lemma pair_in_list_in :
-  forall (l : plist Z) (p1 p2 p3: pointer Z),
+  forall (l : plist R) (p1 p2 p3: pointer R),
     pair_in_list p1 p2 (p3::l) -> In p2 l.
 induction l.
 simpl; tauto.
@@ -688,7 +688,7 @@ intros; subst; intuition.
 intros; intuition.
 subst; intuition.
 right.
-apply IHl with p1 (@null Z).
+apply IHl with p1 (@null R).
 simpl; right; auto.
 Qed.
 
